\documentclass[12pt]{article}
\usepackage{amsmath}
\usepackage{a4wide}
\usepackage{pgf,pgfarrows}
\usepackage[left=2.5cm,right=2.5cm,top=3.5cm,bottom=1.5cm,
            headheight=18pt,headsep=18pt,footskip=24pt,asymmetric=true]{geometry}

\newcommand{\cb}{{\bf c}}
\newcommand{\db}{{\bf d}}
\newcommand{\fb}{{\bf f}}
\newcommand{\gb}{{\bf g}}
\newcommand{\nb}{{\bf n}}
\newcommand{\ub}{{\bf u}}
\newcommand{\vb}{{\bf v}}
\newcommand{\Db}{{\bf D}}
\newcommand{\Kb}{{\bf K}}


\begin{document}

\title{Upscaling notes}
\author{Atgeirr F. Rasmussen}


\section{Notes on anisotropic relperm}

\subsection{The transport equation}

We start from the Darcy equations for each phase, the equation for $p_{cow}$ and the equation for total velocity:
\begin{align}
\vb_\alpha & = -\lambda_\alpha\Kb\nabla p_\alpha + \rho_\alpha\lambda_\alpha\Kb\gb \label{eq:Darcy} \\
\nabla p_{cow} & = \nabla p_o - \nabla p_w \label{eq:GradPcap} \\
\vb & = \vb_o + \vb_w \label{eq:Vtot}
\end{align}

We have 4 equations with 4 unknowns, $\vb_o, \vb_w, \nabla p_o, \nabla p_w$. First, we rewrite the Darcy equations \eqref{eq:Darcy}:
\begin{align*}
 \Kb\nabla p_\alpha & = -\lambda_\alpha^{-1}\vb_\alpha + \rho_\alpha\Kb\gb \\
\end{align*}

Using equation \eqref{eq:GradPcap} we eliminate the phase pressures.
\begin{align*}
 \Kb\nabla p_{cow} & = -\lambda_o^{-1}\vb_o + \rho_o\Kb\gb 
  + \lambda_w^{-1}\vb_w - \rho_w\Kb\gb  \\
  & = -\lambda_o^{-1}\vb_o 
  + \lambda_w^{-1}\vb_w + (\rho_o - \rho_w)\Kb\gb  \\
\end{align*}

Now we use equation \eqref{eq:Vtot} to eliminate $\vb_o$:
\begin{align*}
 \Kb\nabla p_{cow}
  & = -\lambda_o^{-1}\vb + \lambda_o^{-1}\vb_w + \lambda_w^{-1}\vb_w + (\rho_o - \rho_w)\Kb\gb  \\
  (\lambda_o^{-1} + \lambda_w^{-1})\vb_w
  & = \lambda_o^{-1}\vb + \Kb\nabla p_{cow} + (\rho_w - \rho_o)\Kb\gb
\end{align*}

Finally, we achieve a few equivalent equations for $\vb_w$:
\begin{align*}
  \vb_w
  & = \underbrace{\left(I + \lambda_o\lambda_w^{-1}\right)^{-1}}_{\fb_w}
  \left[\vb + \lambda_o\Kb\nabla p_{cow} + (\rho_w - \rho_o)\lambda_o\Kb\gb\right] \\
  \vb_w
  & = \underbrace{\lambda_w\left(\lambda_o + \lambda_w\right)^{-1}}_{\fb_w}
  \left[\vb + \lambda_o\Kb\nabla p_{cow} + (\rho_w - \rho_o)\lambda_o\Kb\gb\right] \\
  \vb_w
  & = \fb_w \vb +
  \underbrace{\lambda_w\left(\lambda_o + \lambda_w\right)^{-1}\lambda_o}_{= \lambda_o^{-1} + \lambda_w^{-1}}
  \Kb\left[\nabla p_{cow} + (\rho_w - \rho_o)\gb\right] \\
\end{align*}

\end{document}
